ram-linear-time/proofs/Lax11Proofs.lean
@@ -5,4 +5,5 @@ import Lax11Proofs.Imp
 import Lax11Proofs.Machine
 import Lax11Proofs.Compile
 import Lax11Proofs.Simulation
+import Lax11Proofs.Reasoning
 import Lax11Proofs.SumSmoke
